nit

steel/Veritas.Steel.MainWorkerChannel.fsti
@@ -9,31 +9,31 @@ module Formats = Veritas.Formats.Types
 module Model = Veritas.Steel.VerifierModel
 module Awc = Veritas.Steel.ApplicationWorkerChannel
 
-// noeq
-// type epoch_hash_entry (c:G.erased Awc.ch) = {
-//   e_id : Formats.epoch_id;
-//   entries : s:G.erased (Seq.seq Formats.vlog_entry){exists n. Awc.sent_s c s n};
-//   hadd : TSM.model_hash;
-//   hevict : h:TSM.model_hash{
-//     let tsm = Model.verify_model (TSM.initial_thread_state_model e_id) entries in
-//     not tsm.TSM.model_failed      /\
-//     tsm.TSM.model_hadd == hadd    /\
-//     tsm.TSM.model_hevict == h};
-// }
-
 val ch : Type0
 
-val reader (c:ch) : vprop
-val writer (c:ch) : vprop
+val reader (c:ch) (a_ch:Awc.ch) : vprop
+val writer (c:ch) (a_ch:Awc.ch) : vprop
 
-val sent (#a_ch:G.erased Awc.ch) (c:ch) (eh:Formats.epoch_hash_entry) : prop
+val sent (c:ch) (a_ch:Awc.ch) (eh:Formats.epoch_hash_entry) : prop
 
-val write (#a_ch:G.erased Awc.ch) (c:ch) (eh:Formats.epoch_hash_entry)
+let valid_epoch_hash_entry (a_ch:Awc.ch) (eh:Formats.epoch_hash_entry) : prop =
+  let open Formats in
+  let open TSM in
+  exists (es:Seq.seq vlog_entry).
+    (exists (n:nat). Awc.sent_s a_ch es n) /\
+    (let tsm = Model.verify_model (initial_thread_state_model (UInt16.v eh.t_id)) es in
+     not tsm.model_failed /\
+     tsm.model_hadd == TSM.bitvec_of_u256 eh.hadd /\
+     tsm.model_hevict == TSM.bitvec_of_u256 eh.hevict)
+
+val write (#a_ch:G.erased Awc.ch)
+  (c:ch)
+  (eh:Formats.epoch_hash_entry{valid_epoch_hash_entry a_ch eh})
   : SteelT bool
-      (writer c)
-      (fun b -> pure (b ==> sent #a_ch c eh) `star` writer c)
+      (writer c a_ch)
+      (fun b -> pure (b ==> sent c a_ch eh) `star` writer c a_ch)
 
 val read (#a_ch:G.erased Awc.ch) (c:ch)
-  : SteelT Formats.epoch_hash_entry
-      (reader c)
-      (fun eh -> pure (sent #a_ch c eh) `star` reader c)
+  : SteelT (eh:Formats.epoch_hash_entry{valid_epoch_hash_entry a_ch eh})
+      (reader c a_ch)
+      (fun eh -> pure (sent c a_ch eh) `star` reader c a_ch)
